theories/SymPolyEnv.v
@@ -10,30 +10,10 @@ Require Import ExtLib.Data.List.
 Require Import ExtLib.Tactics.Consider.
 Require Import MirrorCore.SymI.
 Require Import MirrorCore.TypesI.
+Require Import MirrorCore.Generic.
 
 Set Implicit Arguments.
 Set Strict Implicit.
-
-Section parametric.
-  Fixpoint quant (n : nat) : Type :=
-    match n with
-      | 0 => Type
-      | S n => Type -> quant n
-    end.
-
-  Fixpoint qapply (n : nat) (ls : list Type) : quant n -> Type :=
-    match n as n , ls return quant n -> Type with
-      | 0 , nil => fun t => t
-      | S n , l :: ls => fun f => @qapply n ls (f l)
-      | _ , _ => fun _ => Empty_set
-    end.
-
-  Fixpoint parametric (n : nat) (acc : list Type) (k : list Type -> Type) : Type :=
-    match n with
-      | 0 => k acc
-      | S n => forall T : Type, parametric n (T :: acc) k
-    end.
-End parametric.
 
 Section typed.
   Variable typ : Type.
@@ -176,91 +156,3 @@ Section typed.
        end) ls 1%positive.
 
 End typed.
-
-
-
-(*
-
-  Fixpoint subst0_typ (t : typ) (tv : typ) : typ :=
-    match tv with
-      | tyArr l r => tyArr (subst0_typ t l) (subst0_typ t r)
-      | tyVar 0 => t
-      | tyVar (S n) => tyVar n
-      | tyProp
-      | tyType _ => tv
-    end.
-
-  Theorem typD_subst0_typ : forall acc t l,
-    typD (typD acc l :: acc) t = typD acc (subst0_typ l t).
-  Proof.
-    induction t; try reflexivity.
-    { intros. simpl. rewrite IHt1. rewrite IHt2. reflexivity. }
-    { intros. destruct n; simpl; reflexivity. }
-  Defined.
-
-  (** TODO: I want this **)
-  Definition instantiate_typ (ls : list typ) (tv : typ) : typ :=
-    List.fold_right subst0_typ tv ls.
-
-  Theorem typD_instantiate_typD_cons : forall c t a b,
-    typD (typD b a :: b) (instantiate_typ c t) =
-    typD b (instantiate_typ (a :: c) t).
-  Proof.
-    simpl; intros. rewrite typD_subst0_typ. reflexivity.
-  Defined.
-
-  Fixpoint type_apply n ls acc t {struct n} :
-    parametric n acc (fun env => typD env t) ->
-    option (typD acc (instantiate_typ ls t)) :=
-    match n as n , ls as ls
-      return parametric n acc (fun env => typD env t) ->
-             option (typD acc (instantiate_typ ls t))
-      with
-      | 0 , nil => fun X => Some X
-      | S n , l :: ls => fun X =>
-        match @type_apply n ls _ _ (X (typD acc l)) with
-          | None => None
-          | Some res =>
-            Some match @typD_instantiate_typD_cons _ _ _ _ in _ = t
-                   return t with
-                   | eq_refl => res
-                 end
-        end
-      | _ , _ => fun _ => None
-    end.
-
-  Theorem type_apply_length_equal : forall ft ts' n z fd,
-    length ts' = n ->
-    exists r, type_apply n ts' z ft fd = Some r.
-  Proof.
-    induction ts'; simpl in *; intros; subst; simpl; eauto.
-    match goal with
-      | [ |- exists x, match ?X with _ => _ end = _ ] =>
-        consider X
-    end; intros; eauto.
-    destruct (@IHts' (length ts') (typD z a :: z) (fd (typD z a))
-                     eq_refl).
-    simpl in *.
-    match goal with
-      | [ H : ?X = None , H' : ?Y = Some _ |- _ ] =>
-        let H'' := fresh in
-        assert (H'' : X = Y) by reflexivity; congruence
-    end.
-  Qed.
-
-  Theorem type_apply_length_equal' : forall ft ts' n z fd r,
-    type_apply n ts' z ft fd = Some r ->
-    length ts' = n.
-  Proof.
-    induction ts'; simpl in *; intros; subst; simpl; eauto.
-    { destruct n; simpl in *; auto; congruence. }
-    { destruct n; simpl in *; try congruence.
-      f_equal.
-      match goal with
-        | [ H : match ?X with _ => _ end = _ |- _ ] =>
-          consider X; intros; try congruence
-      end.
-      inversion H0; clear H0; subst. eauto. }
-  Qed.
-
-*)
